examples/low-level/located.fst
@@ -16,9 +16,13 @@ type regionLoc =
 
 assume val regionOf : #a:Type -> located a -> Tot regionLoc
 
-assume val unlocate: #a:Type -> l:(located a){regionOf l = InHeap}  -> Tot a
+assume val lreveal : #a:Type -> l:(located a)  -> Tot (erased a)
 
-assume val locate: #a:Type -> v:a -> Tot (l:(located a){regionOf l= InHeap /\ unlocate l =v})
+val greveal : #a:Type -> l:(located a)  -> GTot a
+let greveal l = reveal (lreveal l)
 
-assume val lreveal : #a:Type -> l:(located a)  -> Tot (v:(erased a){(regionOf l = InHeap) ==> (reveal v = unlocate l)})
 (*for region(stack) allocated stuff, lalloc will have a spec w.r.t reveal*)
+assume val locate: #a:Type -> v:a -> Tot (l:(located a){regionOf l= InHeap /\  greveal l =v})
+
+assume val unlocate: #a:Type -> l:(located a){regionOf l = InHeap}
+  -> Tot (v:a{greveal l =v})
